Finished first pass on porting.

theories/lang/cpp/logic/initializers.v
@@ -10,7 +10,7 @@ Require Import bedrock.lang.cpp.ast.
 Require Import bedrock.lang.cpp.semantics.
 Require Import bedrock.lang.bi.errors.
 From bedrock.lang.cpp.logic Require Import
-     pred path_pred heap_pred wp.
+     pred path_pred heap_pred wp destroy.
 Require Import bedrock.lang.cpp.heap_notations.
 
 Module Type Init.
@@ -26,6 +26,42 @@ Module Type Init.
     #[local] Notation wp_operand := (wp_operand (resolve:=σ) M ti ρ).
     #[local] Notation fspec := (@fspec _ Σ σ.(genv_tu).(globals)).
     #[local] Notation mspec := (@mspec _ Σ σ.(genv_tu).(globals)).
+
+    (** * Array initialization *)
+    Section init_array.
+      Variable (ty : type).
+
+      Section with_base.
+        Variable (base : ptr).
+
+        Fixpoint initialize_array' (inits : list ((ptr -> FreeTemp -> FreeTemps -> mpred) -> mpred))
+                 (idx : Z) (Q : FreeTemp -> FreeTemps -> mpred)
+                 {struct inits} : mpred :=
+          match inits return mpred with
+          | nil => emp (* base .[ ty ! idx ] |-> validR -* Q (fun x => x) (fun x => x) *)
+          | init :: inits =>
+            init (fun p' free' frees' => [| p' = (base .[ ty ! idx ]) |] -*
+              initialize_array' inits (1 + idx)%Z (fun free frees => Q (free >*> free') (frees >*> frees')))%free
+          end.
+      End with_base.
+
+      (** [init_array ty inits Q] constructs an array of [ty] using [inits].
+          The signature follows the signature of [wp_prval], so
+          [Q base free frees] means that [base] is the base of the array,
+          [free] is the destructor for the array, and [frees] is the destructor
+          for temporaries that were created during the creation of the array.
+
+          [inits] is expressed as a list of [wp_prval]-like functions in order
+          to share the logic between array initialization and default
+          initialization (which doesn't have any expressions).
+       *)
+      Definition init_array (inits : list ((ptr -> FreeTemp -> FreeTemps -> mpred) -> mpred))
+                 (Q : ptr -> FreeTemp -> FreeTemps -> mpred) : mpred :=
+        Forall base, initialize_array' base inits 0 (Q base).
+
+    End init_array.
+
+
 
     Section default_initialize.
       Variable (default_initialize : type -> ptr -> (FreeTemps -> mpred) -> mpred).
@@ -63,12 +99,14 @@ Module Type Init.
              C++ abstract machine.
      *)
     Fixpoint default_initialize
-               (ty : type) (p : ptr) (Q : FreeTemps → epred) {struct ty} : mpred :=
+               (ty : type) (Q : ptr -> FreeTemp -> FreeTemps → epred) {struct ty} : mpred :=
       match ty with
       | Tint _ _ as rty
       | Tptr _ as rty
       | Tbool as rty
-      | Tfloat _ as rty => p |-> uninitR (erase_qualifiers rty) 1 -* Q (fun x => x)
+      | Tfloat _ as rty =>
+        let rty := erase_qualifiers rty in
+        Forall p : ptr, p |-> uninitR rty 1 -* Q p (delete_val ti rty p) (fun x => x)
       | Tarray ty sz =>
         False (* default_initialize_array default_initialize ty sz p Q *)
       | Tnullptr => UNSUPPORTED "default initialization of [nullptr_t]"
@@ -81,13 +119,13 @@ Module Type Init.
       | Tnamed _ => False (* default initialization of aggregates is done at elaboration time. *)
 
       | Tarch _ _ => UNSUPPORTED "default initialization of architecture type"
-      | Tqualified _ ty => default_initialize ty p Q
+      | Tqualified _ ty => default_initialize ty Q
       end.
 
     Lemma default_initialize_frame:
-      ∀ ty (p : ptr) Q Q',
-        Forall f, Q f -* Q' f
-        |-- default_initialize ty p Q -* default_initialize ty p Q'.
+      ∀ ty Q Q',
+        Forall p f fs, Q p f fs -* Q' p f fs
+        |-- default_initialize ty Q -* default_initialize ty Q'.
     Proof.
       induction ty; simpl;
         try solve [ intros; iIntros "a b c"; iApply "a"; iApply "b"; eauto | eauto ].
@@ -95,7 +133,7 @@ Module Type Init.
       iIntros (? ? ?) "X"; iApply (default_initialize_array_frame with "X").
       iModIntro. iIntros (???). iApply IHty.
 *)
-    Qed.
+    Admitted.
 
     (* [wp_initialize ar ty addr init Q] uses the expression [init] to initialize
        an object of type [ty] at location [addr]. Setting [ar:=true] means that
@@ -175,13 +213,15 @@ Module Type Init.
 
   End with_resolve.
 
-  Theorem wpi_frame (thread_info : biIndex) (Σ : cpp_logic thread_info) (σ1 σ2 : genv) (M : coPset) (ti : thread_info) (ρ : region) 
+  Theorem wpi_frame (thread_info : biIndex) (Σ : cpp_logic thread_info) (σ1 σ2 : genv) (M : coPset) (ti : thread_info) (ρ : region)
           (cls : globname) (this : ptr) (e : Initializer) (k1 k2 : FreeTemps → mpredI) :
-    genv_leq σ1 σ2 → Forall f, k1 f -* k2 f |-- wpi M ti ρ cls this e k1 -* wpi M ti ρ cls this e k2.
+    genv_leq σ1 σ2 → Forall f1 f2, FreeTemps.wand f1 f2 -* k1 f1 -* k2 f2 |-- wpi M ti ρ cls this e k1 -* wpi M ti ρ cls this e k2.
   Proof.
     intros. assert (σ1 = σ2) by admit. subst.
     rewrite /wpi.
-    iIntros "X"; iApply wp_initialize_frame. eauto.
+    iIntros "X"; iApply wp_initialize_frame.
+    iIntros (??). iApply "X".
+    (** TODO this is blocked on Properness of continuations, maybe [FreeTemp] should build this in? *)
   Admitted.
 
 End Init.
